opentheory/examples/parser.ml
@@ -4,316 +4,316 @@
 
 logfile "parser-stream-def";;
 
-let stream_induct,stream_recursion = define_type
-    "stream = Error
-            | Eof
-            | Stream A stream";;
+let pstream_induct,pstream_recursion = define_type
+    "pstream = ErrorPstream
+             | EofPstream
+             | ConsPstream A pstream";;
 
-export_thm stream_induct;;
-export_thm stream_recursion;;
+export_thm pstream_induct;;
+export_thm pstream_recursion;;
 
-let (case_stream_error,case_stream_eof,case_stream_stream) =
-  let def = new_recursive_definition stream_recursion
-    `(!e b f. case_stream e b f Error = (e:B)) /\
-     (!e b f. case_stream e b f Eof = b) /\
-     (!e b f a s. case_stream e b f (Stream a s) = f (a:A) s)` in
+let (case_pstream_error,case_pstream_eof,case_pstream_cons) =
+  let def = new_recursive_definition pstream_recursion
+    `(!e b f. case_pstream e b f ErrorPstream = (e:B)) /\
+     (!e b f. case_pstream e b f EofPstream = b) /\
+     (!e b f a s. case_pstream e b f (ConsPstream a s) = f (a:A) s)` in
   CONJ_TRIPLE def;;
 
-export_thm case_stream_error;;
-export_thm case_stream_eof;;
-export_thm case_stream_stream;;
+export_thm case_pstream_error;;
+export_thm case_pstream_eof;;
+export_thm case_pstream_cons;;
 
-let case_stream_def =
-  CONJ case_stream_error (CONJ case_stream_eof case_stream_stream);;
+let case_pstream_def =
+  CONJ case_pstream_error (CONJ case_pstream_eof case_pstream_cons);;
 
-let (length_stream_error,length_stream_eof,length_stream_stream) =
-  let def = new_recursive_definition stream_recursion
-    `(length_stream Error = 0) /\
-     (length_stream Eof = 0) /\
-     (!(a:A) s. length_stream (Stream a s) = SUC (length_stream s))` in
+let (length_pstream_error,length_pstream_eof,length_pstream_cons) =
+  let def = new_recursive_definition pstream_recursion
+    `(length_pstream ErrorPstream = 0) /\
+     (length_pstream EofPstream = 0) /\
+     (!(a:A) s. length_pstream (ConsPstream a s) = SUC (length_pstream s))` in
   CONJ_TRIPLE def;;
 
-export_thm length_stream_error;;
-export_thm length_stream_eof;;
-export_thm length_stream_stream;;
+export_thm length_pstream_error;;
+export_thm length_pstream_eof;;
+export_thm length_pstream_cons;;
 
-let length_stream_def =
-  CONJ length_stream_error (CONJ length_stream_eof length_stream_stream);;
+let length_pstream_def =
+  CONJ length_pstream_error (CONJ length_pstream_eof length_pstream_cons);;
 
-let (is_proper_suffix_stream_error,
-     is_proper_suffix_stream_eof,
-     is_proper_suffix_stream_stream) =
-  let def = new_recursive_definition stream_recursion
-  `(!s. is_proper_suffix_stream s Error = F) /\
-   (!s. is_proper_suffix_stream s Eof = F) /\
-   (!s a s'. is_proper_suffix_stream s (Stream (a:A) s') =
-      ((s = s') \/ is_proper_suffix_stream s s'))` in
+let (is_proper_suffix_pstream_error,
+     is_proper_suffix_pstream_eof,
+     is_proper_suffix_pstream_cons) =
+  let def = new_recursive_definition pstream_recursion
+  `(!s. is_proper_suffix_pstream s ErrorPstream = F) /\
+   (!s. is_proper_suffix_pstream s EofPstream = F) /\
+   (!s a s'. is_proper_suffix_pstream s (ConsPstream (a:A) s') =
+      ((s = s') \/ is_proper_suffix_pstream s s'))` in
    CONJ_TRIPLE (REWRITE_RULE [] def);;
 
-export_thm is_proper_suffix_stream_error;;
-export_thm is_proper_suffix_stream_eof;;
-export_thm is_proper_suffix_stream_stream;;
+export_thm is_proper_suffix_pstream_error;;
+export_thm is_proper_suffix_pstream_eof;;
+export_thm is_proper_suffix_pstream_cons;;
 
-let is_proper_suffix_stream_def =
-  CONJ is_proper_suffix_stream_error
-    (CONJ is_proper_suffix_stream_eof is_proper_suffix_stream_stream);;
+let is_proper_suffix_pstream_def =
+  CONJ is_proper_suffix_pstream_error
+    (CONJ is_proper_suffix_pstream_eof is_proper_suffix_pstream_cons);;
 
-let is_suffix_stream_def = new_definition
+let is_suffix_pstream_def = new_definition
   `!s s'.
-     is_suffix_stream s s' =
-     (((s : A stream) = s') \/ is_proper_suffix_stream s s')`;;
+     is_suffix_pstream s s' =
+     (((s : A pstream) = s') \/ is_proper_suffix_pstream s s')`;;
 
-export_thm is_suffix_stream_def;;
+export_thm is_suffix_pstream_def;;
 
-let (stream_to_list_error,
-     stream_to_list_eof,
-     stream_to_list_stream) =
-  let def = new_recursive_definition stream_recursion
-    `(stream_to_list Error = NONE) /\
-     (stream_to_list Eof = SOME []) /\
-     (!a s. stream_to_list (Stream a s) =
+let (pstream_to_list_error,
+     pstream_to_list_eof,
+     pstream_to_list_cons) =
+  let def = new_recursive_definition pstream_recursion
+    `(pstream_to_list ErrorPstream = NONE) /\
+     (pstream_to_list EofPstream = SOME []) /\
+     (!a s. pstream_to_list (ConsPstream a s) =
         case_option
           NONE
           (\l. SOME (CONS (a:A) l))
-          (stream_to_list s))` in
+          (pstream_to_list s))` in
   CONJ_TRIPLE def;;
 
-export_thm stream_to_list_error;;
-export_thm stream_to_list_eof;;
-export_thm stream_to_list_stream;;
+export_thm pstream_to_list_error;;
+export_thm pstream_to_list_eof;;
+export_thm pstream_to_list_cons;;
 
-let stream_to_list_def =
-  CONJ stream_to_list_error
-    (CONJ stream_to_list_eof stream_to_list_stream);;
+let pstream_to_list_def =
+  CONJ pstream_to_list_error
+    (CONJ pstream_to_list_eof pstream_to_list_cons);;
 
-let (append_stream_nil,append_stream_cons) =
+let (append_pstream_nil,append_pstream_cons) =
   let def = new_recursive_definition list_RECURSION
-    `(!s. append_stream [] s = s) /\
-     (!h t s. append_stream (CONS h t) s = Stream (h:A) (append_stream t s))` in
+    `(!s. append_pstream [] s = s) /\
+     (!h t s. append_pstream (CONS h t) s = ConsPstream (h:A) (append_pstream t s))` in
   CONJ_PAIR def;;
 
-export_thm append_stream_nil;;
-export_thm append_stream_cons;;
+export_thm append_pstream_nil;;
+export_thm append_pstream_cons;;
 
-let append_stream_def = CONJ append_stream_nil append_stream_cons;;
+let append_pstream_def = CONJ append_pstream_nil append_pstream_cons;;
 
-let list_to_stream_def = new_definition
-  `!(l : A list). list_to_stream l = append_stream l Eof`;;
+let list_to_pstream_def = new_definition
+  `!(l : A list). list_to_pstream l = append_pstream l EofPstream`;;
 
-export_thm list_to_stream_def;;
+export_thm list_to_pstream_def;;
 
 logfile "parser-stream-thm";;
 
-let stream_cases = prove_cases_thm stream_induct;;
+let pstream_cases = prove_cases_thm pstream_induct;;
 
-export_thm stream_cases;;
+export_thm pstream_cases;;
 
-let (stream_distinct_error_eof,
-     stream_distinct_error_stream,
-     stream_distinct_eof_stream) =
-    CONJ_TRIPLE (distinctness "stream");;
+let (pstream_distinct_error_eof,
+     pstream_distinct_error_cons,
+     pstream_distinct_eof_cons) =
+    CONJ_TRIPLE (distinctness "pstream");;
 
-export_thm stream_distinct_error_eof;;
-export_thm stream_distinct_error_stream;;
-export_thm stream_distinct_eof_stream;;
+export_thm pstream_distinct_error_eof;;
+export_thm pstream_distinct_error_cons;;
+export_thm pstream_distinct_eof_cons;;
 
-let stream_distinct =
-    CONJ stream_distinct_error_eof
-      (CONJ stream_distinct_error_stream stream_distinct_eof_stream);;
+let pstream_distinct =
+    CONJ pstream_distinct_error_eof
+      (CONJ pstream_distinct_error_cons pstream_distinct_eof_cons);;
 
-let stream_inj = injectivity "stream";;
+let pstream_inj = injectivity "pstream";;
 
-export_thm stream_inj;;
+export_thm pstream_inj;;
 
-let is_proper_suffix_stream_trans = prove
-  (`!x y z : A stream.
-      is_proper_suffix_stream x y /\ is_proper_suffix_stream y z ==>
-      is_proper_suffix_stream x z`,
+let is_proper_suffix_pstream_trans = prove
+  (`!x y z : A pstream.
+      is_proper_suffix_pstream x y /\ is_proper_suffix_pstream y z ==>
+      is_proper_suffix_pstream x z`,
    GEN_TAC THEN
    GEN_TAC THEN
-   MATCH_MP_TAC stream_induct THEN
-   ASM_REWRITE_TAC [is_proper_suffix_stream_def] THEN
+   MATCH_MP_TAC pstream_induct THEN
+   ASM_REWRITE_TAC [is_proper_suffix_pstream_def] THEN
    REPEAT STRIP_TAC THEN
    ASM_MESON_TAC []);;
 
-export_thm is_proper_suffix_stream_trans;;
+export_thm is_proper_suffix_pstream_trans;;
 
-let is_proper_suffix_stream_length = prove
-  (`!x y : A stream.
-      is_proper_suffix_stream x y ==> length_stream x < length_stream y`,
+let is_proper_suffix_pstream_length = prove
+  (`!x y : A pstream.
+      is_proper_suffix_pstream x y ==> length_pstream x < length_pstream y`,
    GEN_TAC THEN
-   MATCH_MP_TAC stream_induct THEN
+   MATCH_MP_TAC pstream_induct THEN
    ASM_REWRITE_TAC
-     [is_proper_suffix_stream_def; length_stream_def; LT_SUC_LE] THEN
+     [is_proper_suffix_pstream_def; length_pstream_def; LT_SUC_LE] THEN
    REPEAT STRIP_TAC THEN
    ASM_MESON_TAC [LE_REFL; LT_IMP_LE]);;
 
-export_thm is_proper_suffix_stream_length;;
+export_thm is_proper_suffix_pstream_length;;
 
-let is_proper_suffix_stream_wf = prove
-  (`WF (is_proper_suffix_stream : A stream -> A stream -> bool)`,
+let is_proper_suffix_pstream_wf = prove
+  (`WF (is_proper_suffix_pstream : A pstream -> A pstream -> bool)`,
    MATCH_MP_TAC
-     (ISPECL [`is_proper_suffix_stream : A stream -> A stream -> bool`;
-              `MEASURE (length_stream : A stream -> num)`] WF_SUBSET) THEN
+     (ISPECL [`is_proper_suffix_pstream : A pstream -> A pstream -> bool`;
+              `MEASURE (length_pstream : A pstream -> num)`] WF_SUBSET) THEN
    REWRITE_TAC [WF_MEASURE] THEN
-   REWRITE_TAC [MEASURE; is_proper_suffix_stream_length]);;
+   REWRITE_TAC [MEASURE; is_proper_suffix_pstream_length]);;
 
-export_thm is_proper_suffix_stream_wf;;
+export_thm is_proper_suffix_pstream_wf;;
 
-let is_proper_suffix_stream_refl = prove
-  (`!x : A stream. ~is_proper_suffix_stream x x`,
+let is_proper_suffix_pstream_refl = prove
+  (`!x : A pstream. ~is_proper_suffix_pstream x x`,
    GEN_TAC THEN
    MATCH_MP_TAC WF_REFL THEN
-   ACCEPT_TAC is_proper_suffix_stream_wf);;
+   ACCEPT_TAC is_proper_suffix_pstream_wf);;
 
-export_thm is_proper_suffix_stream_refl;;
+export_thm is_proper_suffix_pstream_refl;;
 
-let is_proper_suffix_stream_induct = prove
-  (`!(p : A stream -> bool).
-       (!x. (!y. is_proper_suffix_stream y x ==> p y) ==> p x) ==> !x. p x`,
-   REWRITE_TAC [GSYM WF_IND; is_proper_suffix_stream_wf]);;
+let is_proper_suffix_pstream_induct = prove
+  (`!(p : A pstream -> bool).
+       (!x. (!y. is_proper_suffix_pstream y x ==> p y) ==> p x) ==> !x. p x`,
+   REWRITE_TAC [GSYM WF_IND; is_proper_suffix_pstream_wf]);;
 
-export_thm is_proper_suffix_stream_induct;;
+export_thm is_proper_suffix_pstream_induct;;
 
-let is_proper_suffix_stream_recursion = prove
-  (`!(h : (A stream -> B) -> A stream -> B).
+let is_proper_suffix_pstream_recursion = prove
+  (`!(h : (A pstream -> B) -> A pstream -> B).
        (!f g s.
-          (!s'. is_proper_suffix_stream s' s ==> (f s' = g s')) ==>
+          (!s'. is_proper_suffix_pstream s' s ==> (f s' = g s')) ==>
           (h f s = h g s)) ==>
        ?f. !s. f s = h f s`,
    MATCH_MP_TAC WF_REC THEN
-   REWRITE_TAC [is_proper_suffix_stream_wf]);;
+   REWRITE_TAC [is_proper_suffix_pstream_wf]);;
 
-export_thm is_proper_suffix_stream_recursion;;
+export_thm is_proper_suffix_pstream_recursion;;
 
-let is_suffix_stream_proper = prove
-  (`!x y : A stream. is_proper_suffix_stream x y ==> is_suffix_stream x y`,
-   SIMP_TAC [is_suffix_stream_def]);;
+let is_suffix_pstream_proper = prove
+  (`!x y : A pstream. is_proper_suffix_pstream x y ==> is_suffix_pstream x y`,
+   SIMP_TAC [is_suffix_pstream_def]);;
 
-export_thm is_suffix_stream_proper;;
+export_thm is_suffix_pstream_proper;;
 
-let is_suffix_stream_refl = prove
-  (`!x : A stream. is_suffix_stream x x`,
-   SIMP_TAC [is_suffix_stream_def]);;
+let is_suffix_pstream_refl = prove
+  (`!x : A pstream. is_suffix_pstream x x`,
+   SIMP_TAC [is_suffix_pstream_def]);;
 
-export_thm is_suffix_stream_refl;;
+export_thm is_suffix_pstream_refl;;
 
-let is_suffix_stream_trans = prove
-  (`!x y z : A stream.
-      is_suffix_stream x y /\ is_suffix_stream y z ==>
-      is_suffix_stream x z`,
+let is_suffix_pstream_trans = prove
+  (`!x y z : A pstream.
+      is_suffix_pstream x y /\ is_suffix_pstream y z ==>
+      is_suffix_pstream x z`,
    REPEAT GEN_TAC THEN
-   REWRITE_TAC [is_suffix_stream_def] THEN
+   REWRITE_TAC [is_suffix_pstream_def] THEN
    STRIP_TAC THEN
    ASM_REWRITE_TAC [] THEN
-   ASM_MESON_TAC [is_proper_suffix_stream_trans]);;
+   ASM_MESON_TAC [is_proper_suffix_pstream_trans]);;
 
-export_thm is_suffix_stream_trans;;
+export_thm is_suffix_pstream_trans;;
 
-let append_stream_assoc = prove
-  (`!x y z : A stream.
-      append_stream (APPEND x y) z = append_stream x (append_stream y z)`,
+let append_pstream_assoc = prove
+  (`!x y z : A pstream.
+      append_pstream (APPEND x y) z = append_pstream x (append_pstream y z)`,
    LIST_INDUCT_TAC THEN
-   ASM_REWRITE_TAC [APPEND; append_stream_def]);;
+   ASM_REWRITE_TAC [APPEND; append_pstream_def]);;
 
-export_thm append_stream_assoc;;
+export_thm append_pstream_assoc;;
 
-let list_to_stream_to_list = prove
-  (`!l : A list. stream_to_list (list_to_stream l) = SOME l`,
-   REWRITE_TAC [list_to_stream_def] THEN
+let list_to_pstream_to_list = prove
+  (`!l : A list. pstream_to_list (list_to_pstream l) = SOME l`,
+   REWRITE_TAC [list_to_pstream_def] THEN
    LIST_INDUCT_TAC THENL
-   [REWRITE_TAC [stream_to_list_def; append_stream_def];
-    REWRITE_TAC [stream_to_list_def; append_stream_def] THEN
+   [REWRITE_TAC [pstream_to_list_def; append_pstream_def];
+    REWRITE_TAC [pstream_to_list_def; append_pstream_def] THEN
     ASM_REWRITE_TAC [case_option_def]]);;
 
-export_thm list_to_stream_to_list;;
+export_thm list_to_pstream_to_list;;
 
-let stream_to_list_append = prove
+let pstream_to_list_append = prove
   (`!(l : A list) s.
-      stream_to_list (append_stream l s) =
-      case_option NONE (\ls. SOME (APPEND l ls)) (stream_to_list s)`,
+      pstream_to_list (append_pstream l s) =
+      case_option NONE (\ls. SOME (APPEND l ls)) (pstream_to_list s)`,
    LIST_INDUCT_TAC THENL
-   [REWRITE_TAC [APPEND; append_stream_def] THEN
+   [REWRITE_TAC [APPEND; append_pstream_def] THEN
     CONV_TAC (DEPTH_CONV ETA_CONV) THEN
     REWRITE_TAC [case_option_id];
     ALL_TAC] THEN
    GEN_TAC THEN
-   REWRITE_TAC [APPEND; append_stream_def; stream_to_list_def] THEN
+   REWRITE_TAC [APPEND; append_pstream_def; pstream_to_list_def] THEN
    POP_ASSUM (fun th -> REWRITE_TAC [th]) THEN
-   MP_TAC (ISPEC `stream_to_list (s : A stream)` option_cases) THEN
+   MP_TAC (ISPEC `pstream_to_list (s : A pstream)` option_cases) THEN
    STRIP_TAC THENL
    [ASM_REWRITE_TAC [case_option_def];
     ASM_REWRITE_TAC [case_option_def]]);;
 
-export_thm stream_to_list_append;;
+export_thm pstream_to_list_append;;
 
-let is_suffix_stream_length = prove
-  (`!x y : A stream.
-      is_suffix_stream x y ==> length_stream x <= length_stream y`,
-   REWRITE_TAC [is_suffix_stream_def; LE_LT] THEN
+let is_suffix_pstream_length = prove
+  (`!x y : A pstream.
+      is_suffix_pstream x y ==> length_pstream x <= length_pstream y`,
+   REWRITE_TAC [is_suffix_pstream_def; LE_LT] THEN
    REPEAT STRIP_TAC THENL
    [DISJ2_TAC THEN
     ASM_REWRITE_TAC [];
     DISJ1_TAC THEN
-    MATCH_MP_TAC is_proper_suffix_stream_length THEN
+    MATCH_MP_TAC is_proper_suffix_pstream_length THEN
     FIRST_ASSUM ACCEPT_TAC]);;
 
-export_thm is_suffix_stream_length;;
+export_thm is_suffix_pstream_length;;
 
-let append_stream_length = prove
+let append_pstream_length = prove
   (`!(l : A list) s.
-      length_stream (append_stream l s) = LENGTH l + length_stream s`,
+      length_pstream (append_pstream l s) = LENGTH l + length_pstream s`,
    LIST_INDUCT_TAC THENL
-   [REWRITE_TAC [length_stream_def; append_stream_def; LENGTH; ADD];
-    ASM_REWRITE_TAC [length_stream_def; append_stream_def; LENGTH; ADD]]);;
+   [REWRITE_TAC [length_pstream_def; append_pstream_def; LENGTH; ADD];
+    ASM_REWRITE_TAC [length_pstream_def; append_pstream_def; LENGTH; ADD]]);;
 
-export_thm append_stream_length;;
+export_thm append_pstream_length;;
 
-let list_to_stream_length = prove
-  (`!l : A list. length_stream (list_to_stream l) = LENGTH l`,
+let list_to_pstream_length = prove
+  (`!l : A list. length_pstream (list_to_pstream l) = LENGTH l`,
    REWRITE_TAC
-     [list_to_stream_def; append_stream_length; length_stream_def; ADD_0]);;
+     [list_to_pstream_def; append_pstream_length; length_pstream_def; ADD_0]);;
 
-export_thm list_to_stream_length;;
+export_thm list_to_pstream_length;;
 
-let stream_to_list_length = prove
-  (`!s : A stream.
-     case_option T (\l. LENGTH l = length_stream s) (stream_to_list s)`,
-   MATCH_MP_TAC stream_induct THEN
+let pstream_to_list_length = prove
+  (`!s : A pstream.
+     case_option T (\l. LENGTH l = length_pstream s) (pstream_to_list s)`,
+   MATCH_MP_TAC pstream_induct THEN
    CONJ_TAC THENL
-   [REWRITE_TAC [stream_to_list_def; case_option_def];
+   [REWRITE_TAC [pstream_to_list_def; case_option_def];
     ALL_TAC] THEN
    CONJ_TAC THENL
    [REWRITE_TAC
-      [stream_to_list_def; case_option_def; LENGTH; length_stream_def];
+      [pstream_to_list_def; case_option_def; LENGTH; length_pstream_def];
     ALL_TAC] THEN
    REPEAT GEN_TAC THEN
-   REWRITE_TAC [stream_to_list_def] THEN
-   MP_TAC (ISPEC `stream_to_list (a1 : A stream)` option_cases) THEN
+   REWRITE_TAC [pstream_to_list_def] THEN
+   MP_TAC (ISPEC `pstream_to_list (a1 : A pstream)` option_cases) THEN
    STRIP_TAC THENL
    [ASM_REWRITE_TAC [case_option_def];
     ALL_TAC] THEN
    ASM_REWRITE_TAC [case_option_def] THEN
-   REWRITE_TAC [LENGTH; length_stream_def; SUC_INJ]);;
+   REWRITE_TAC [LENGTH; length_pstream_def; SUC_INJ]);;
 
-export_thm stream_to_list_length;;
+export_thm pstream_to_list_length;;
 
 logfile "parser-comb-def";;
 
 let is_parser_def = new_definition
-  `!(p : A -> A stream -> (B # A stream) option).
+  `!(p : A -> A pstream -> (B # A pstream) option).
      is_parser p <=>
        !x xs.
          case_option
            T
-           (\ (y,xs'). is_suffix_stream xs' xs)
+           (\ (y,xs'). is_suffix_pstream xs' xs)
            (p x xs)`;;
 
 export_thm is_parser_def;;
 
 let parser_exists = prove
-  (`?(p : A -> A stream -> (B # A stream) option). is_parser p`,
-   EXISTS_TAC `\(x:A) (s:A stream). (NONE : (B # A stream) option)` THEN
+  (`?(p : A -> A pstream -> (B # A pstream) option). is_parser p`,
+   EXISTS_TAC `\(x:A) (s:A pstream). (NONE : (B # A pstream) option)` THEN
    REWRITE_TAC [is_parser_def; case_option_def]);;
 
 let (parser_abs_rep,parser_rep_abs) =
@@ -326,25 +326,25 @@ export_thm parser_rep_abs;;
 
 let parser_tybij = CONJ parser_abs_rep parser_rep_abs;;
 
-let (parse_error,parse_eof,parse_stream) =
-  let def = new_recursive_definition stream_recursion
-    `(!p : (A,B) parser. parse p Error = NONE) /\
-     (!p : (A,B) parser. parse p Eof = NONE) /\
-     (!p : (A,B) parser. !a s. parse p (Stream a s) = dest_parser p a s)` in
+let (parse_error,parse_eof,parse_cons) =
+  let def = new_recursive_definition pstream_recursion
+    `(!p : (A,B) parser. parse p ErrorPstream = NONE) /\
+     (!p : (A,B) parser. parse p EofPstream = NONE) /\
+     (!p : (A,B) parser. !a s. parse p (ConsPstream a s) = dest_parser p a s)` in
   CONJ_TRIPLE def;;
 
 export_thm parse_error;;
 export_thm parse_eof;;
-export_thm parse_stream;;
+export_thm parse_cons;;
 
 let parse_def =
   REWRITE_RULE [GSYM FORALL_AND_THM]
-    (CONJ parse_error (CONJ parse_eof parse_stream));;
+    (CONJ parse_error (CONJ parse_eof parse_cons));;
 
 let parse_inverse_def = new_definition
   `!p e.
      parse_inverse p (e : B -> A list) <=>
-     !x s. parse p (append_stream (e x) s) = SOME (x,s)`;;
+     !x s. parse p (append_pstream (e x) s) = SOME (x,s)`;;
 
 export_thm parse_inverse_def;;
 
@@ -352,12 +352,12 @@ let parse_strong_inverse_def = new_definition
   `!p e.
      parse_strong_inverse p (e : B -> A list) <=>
      parse_inverse p e /\
-     !s x s'. parse p s = SOME (x,s') ==> s = append_stream (e x) s'`;;
+     !s x s'. parse p s = SOME (x,s') ==> s = append_pstream (e x) s'`;;
 
 export_thm parse_strong_inverse_def;;
 
 let parser_none_def = new_definition
-  `!a s. parser_none (a : A) (s : A stream) = (NONE : (B # A stream) option)`;;
+  `!a s. parser_none (a : A) (s : A pstream) = (NONE : (B # A pstream) option)`;;
 
 export_thm parser_none_def;;
 
@@ -367,7 +367,7 @@ let parse_none_def = new_definition
 export_thm parse_none_def;;
 
 let parser_all_def = new_definition
-  `!a s. parser_all (a : A) (s : A stream) = SOME (a,s)`;;
+  `!a s. parser_all (a : A) (s : A pstream) = SOME (a,s)`;;
 
 export_thm parser_all_def;;
 
@@ -442,25 +442,25 @@ let dest_is_parser = prove
 export_thm dest_is_parser;;
 
 let is_parser_cases = prove
-  (`!(p : A -> A stream -> (B # A stream) option) a s.
+  (`!(p : A -> A pstream -> (B # A pstream) option) a s.
        is_parser p ==>
        (p a s = NONE) \/
-       (?b s'. p a s = SOME (b,s') /\ is_suffix_stream s' s)`,
+       (?b s'. p a s = SOME (b,s') /\ is_suffix_pstream s' s)`,
    REPEAT GEN_TAC THEN
    REWRITE_TAC [is_parser_def] THEN
-   DISCH_THEN (MP_TAC o SPECL [`a:A`;`s:A stream`]) THEN
+   DISCH_THEN (MP_TAC o SPECL [`a:A`;`s:A pstream`]) THEN
    MP_TAC
-     (ISPEC `(p : A -> A stream -> (B # A stream) option) a s`
+     (ISPEC `(p : A -> A pstream -> (B # A pstream) option) a s`
         option_cases) THEN
    STRIP_TAC THEN
    ASM_REWRITE_TAC [case_option_def] THEN
-   MP_TAC (ISPEC `a' : B # A stream` PAIR_SURJECTIVE) THEN
+   MP_TAC (ISPEC `a' : B # A pstream` PAIR_SURJECTIVE) THEN
    STRIP_TAC THEN
    ASM_REWRITE_TAC [] THEN
    STRIP_TAC THEN
    DISJ2_TAC THEN
    EXISTS_TAC `x:B` THEN
-   EXISTS_TAC `y:A stream` THEN
+   EXISTS_TAC `y:A pstream` THEN
    ASM_REWRITE_TAC []);;
 
 export_thm is_parser_cases;;
@@ -468,49 +468,49 @@ export_thm is_parser_cases;;
 let dest_parser_cases = prove
   (`!(p : (A,B) parser) a s.
        (dest_parser p a s = NONE) \/
-       (?b s'. dest_parser p a s = SOME (b,s') /\ is_suffix_stream s' s)`,
+       (?b s'. dest_parser p a s = SOME (b,s') /\ is_suffix_pstream s' s)`,
    REPEAT GEN_TAC THEN
-   MP_TAC (SPECL [`dest_parser (p : (A,B) parser)`; `a:A`; `s:A stream`]
+   MP_TAC (SPECL [`dest_parser (p : (A,B) parser)`; `a:A`; `s:A pstream`]
              is_parser_cases) THEN
    REWRITE_TAC [dest_is_parser]);;
 
 export_thm dest_parser_cases;;
 
-let dest_parser_suffix_stream = prove
+let dest_parser_suffix_pstream = prove
   (`!(p : (A,B) parser) a s b s'.
-       dest_parser p a s = SOME (b,s') ==> is_suffix_stream s' s`,
+       dest_parser p a s = SOME (b,s') ==> is_suffix_pstream s' s`,
    REPEAT GEN_TAC THEN
    STRIP_TAC THEN
-   MP_TAC (SPECL [`p : (A,B) parser`; `a:A`; `s:A stream`]
+   MP_TAC (SPECL [`p : (A,B) parser`; `a:A`; `s:A pstream`]
              dest_parser_cases) THEN
    ASM_REWRITE_TAC [option_distinct; option_inj; PAIR_EQ] THEN
    STRIP_TAC THEN
    ASM_REWRITE_TAC []);;
 
-export_thm dest_parser_suffix_stream;;
+export_thm dest_parser_suffix_pstream;;
 
 let parse_cases = prove
   (`!(p : (A,B) parser) s.
        (parse p s = NONE) \/
-       (?b s'. parse p s = SOME (b,s') /\ is_proper_suffix_stream s' s)`,
+       (?b s'. parse p s = SOME (b,s') /\ is_proper_suffix_pstream s' s)`,
    REPEAT GEN_TAC THEN
-   MP_TAC (ISPEC `s : A stream` stream_cases) THEN
+   MP_TAC (ISPEC `s : A pstream` pstream_cases) THEN
    STRIP_TAC THEN
    ASM_REWRITE_TAC [parse_def] THEN
-   MP_TAC (SPECL [`p : (A,B) parser`; `a0 : A`; `a1 : A stream`]
+   MP_TAC (SPECL [`p : (A,B) parser`; `a0 : A`; `a1 : A pstream`]
              dest_parser_cases) THEN
-   REWRITE_TAC [is_suffix_stream_def] THEN
+   REWRITE_TAC [is_suffix_pstream_def] THEN
    STRIP_TAC THEN
    ASM_REWRITE_TAC [] THEN
    DISJ2_TAC THEN
    EXISTS_TAC `b : B` THEN
-   EXISTS_TAC `s' : A stream` THEN
-   ASM_REWRITE_TAC [is_proper_suffix_stream_def]);;
+   EXISTS_TAC `s' : A pstream` THEN
+   ASM_REWRITE_TAC [is_proper_suffix_pstream_def]);;
 
 export_thm parse_cases;;
 
 let is_parser_none = prove
-  (`is_parser (parser_none : A -> A stream -> (B # A stream) option)`,
+  (`is_parser (parser_none : A -> A pstream -> (B # A pstream) option)`,
    REWRITE_TAC [is_parser_def; parser_none_def; case_option_def]);;
 
 export_thm is_parser_none;;
@@ -525,17 +525,17 @@ export_thm dest_parse_none;;
 let parse_parse_none = prove
   (`!s. parse (parse_none : (A,B) parser) s = NONE`,
     REPEAT STRIP_TAC THEN
-    MP_TAC (ISPEC `s : A stream` stream_cases) THEN
+    MP_TAC (ISPEC `s : A pstream` pstream_cases) THEN
     REPEAT STRIP_TAC THEN
-    ASM_REWRITE_TAC [parse_def; case_stream_def; case_option_def] THEN
+    ASM_REWRITE_TAC [parse_def; case_pstream_def; case_option_def] THEN
     REWRITE_TAC [dest_parse_none; parser_none_def]);;
 
 export_thm parse_parse_none;;
 
 let is_parser_all = prove
-  (`is_parser (parser_all : A -> A stream -> (A # A stream) option)`,
+  (`is_parser (parser_all : A -> A pstream -> (A # A pstream) option)`,
    REWRITE_TAC
-     [is_parser_def; parser_all_def; case_option_def; is_suffix_stream_refl]);;
+     [is_parser_def; parser_all_def; case_option_def; is_suffix_pstream_refl]);;
 
 export_thm is_parser_all;;
 
@@ -548,12 +548,12 @@ export_thm dest_parse_none;;
 
 let parse_parse_all = prove
   (`parse (parse_all : (A,A) parser) =
-    case_stream NONE NONE (\a s. SOME (a,s))`,
+    case_pstream NONE NONE (\a s. SOME (a,s))`,
     ONCE_REWRITE_TAC [FUN_EQ_THM] THEN
     REPEAT STRIP_TAC THEN
-    MP_TAC (ISPEC `x : A stream` stream_cases) THEN
+    MP_TAC (ISPEC `x : A pstream` pstream_cases) THEN
     REPEAT STRIP_TAC THEN
-    ASM_REWRITE_TAC [parse_def; case_stream_def; case_option_def] THEN
+    ASM_REWRITE_TAC [parse_def; case_pstream_def; case_option_def] THEN
     REWRITE_TAC [dest_parse_all; parser_all_def]);;
 
 export_thm parse_parse_all;;
@@ -563,7 +563,7 @@ let parse_all_inverse = prove
    REWRITE_TAC [parse_inverse_def] THEN
    REPEAT STRIP_TAC THEN
    ASM_REWRITE_TAC
-     [parse_parse_all; append_stream_def; case_stream_def;
+     [parse_parse_all; append_pstream_def; case_pstream_def;
       case_option_def]);;
 
 export_thm parse_all_inverse;;
@@ -571,12 +571,12 @@ export_thm parse_all_inverse;;
 let parse_all_strong_inverse = prove
   (`parse_strong_inverse (parse_all : (A,A) parser) (\a. CONS a [])`,
    REWRITE_TAC [parse_strong_inverse_def; parse_all_inverse] THEN
-   ASM_REWRITE_TAC [parse_parse_all; append_stream_def] THEN
+   ASM_REWRITE_TAC [parse_parse_all; append_pstream_def] THEN
    REPEAT GEN_TAC THEN
-   MP_TAC (ISPEC `s : A stream` stream_cases) THEN
+   MP_TAC (ISPEC `s : A pstream` pstream_cases) THEN
    STRIP_TAC THEN
    ASM_REWRITE_TAC
-     [case_stream_def; option_distinct; stream_inj; option_inj; PAIR_EQ]);;
+     [case_pstream_def; option_distinct; pstream_inj; option_inj; PAIR_EQ]);;
 
 export_thm parse_all_strong_inverse;;
 
@@ -586,7 +586,7 @@ let is_parser_partial_map = prove
    REWRITE_TAC [is_parser_def; parser_partial_map_def] THEN
    REPEAT GEN_TAC THEN
    MP_TAC (ISPECL [`p : (A,B) parser`;
-                   `x : A`; `xs : A stream`] dest_parser_cases) THEN
+                   `x : A`; `xs : A pstream`] dest_parser_cases) THEN
    STRIP_TAC THEN
    ASM_REWRITE_TAC [case_option_def] THEN
    MP_TAC (ISPECL [`(f : B -> C option) b`] option_cases) THEN
@@ -614,7 +614,7 @@ let parse_parse_partial_map = prove
         (\ (b,s'). case_option NONE (\c. SOME (c,s')) (f b))
         (parse p s)`,
     REPEAT GEN_TAC THEN
-    MP_TAC (ISPEC `s : A stream` stream_cases) THEN
+    MP_TAC (ISPEC `s : A pstream` pstream_cases) THEN
     REPEAT STRIP_TAC THEN
     ASM_REWRITE_TAC [parse_def; case_option_def] THEN
     REWRITE_TAC [dest_parse_partial_map; parser_partial_map_def]);;
@@ -629,7 +629,7 @@ let parse_partial_map_inverse = prove
    REWRITE_TAC [parse_inverse_def] THEN
    REPEAT STRIP_TAC THEN
    ASM_REWRITE_TAC
-     [parse_parse_partial_map; append_stream_def; case_stream_def;
+     [parse_parse_partial_map; append_pstream_def; case_pstream_def;
       case_option_def]);;
 
 export_thm parse_partial_map_inverse;;
@@ -645,8 +645,8 @@ let parse_partial_map_strong_inverse = prove
    [MATCH_MP_TAC parse_partial_map_inverse THEN
     ASM_REWRITE_TAC [];
     POP_ASSUM MP_TAC THEN
-    ASM_REWRITE_TAC [parse_parse_partial_map; append_stream_def] THEN
-    MP_TAC (ISPECL [`p : (A,B) parser`; `s : A stream`] parse_cases) THEN
+    ASM_REWRITE_TAC [parse_parse_partial_map; append_pstream_def] THEN
+    MP_TAC (ISPECL [`p : (A,B) parser`; `s : A pstream`] parse_cases) THEN
     STRIP_TAC THEN
     ASM_REWRITE_TAC [case_option_def; option_distinct; option_inj; PAIR_EQ] THEN
     MP_TAC (ISPEC `(f : B -> C option) b` option_cases) THEN
@@ -694,7 +694,7 @@ let parse_map_inverse = prove
    REWRITE_TAC [parse_inverse_def] THEN
    REPEAT STRIP_TAC THEN
    ASM_REWRITE_TAC
-     [parse_parse_map; append_stream_def; case_stream_def;
+     [parse_parse_map; append_pstream_def; case_pstream_def;
       case_option_def]);;
 
 export_thm parse_map_inverse;;
@@ -710,8 +710,8 @@ let parse_map_strong_inverse = prove
    [MATCH_MP_TAC parse_map_inverse THEN
     ASM_REWRITE_TAC [];
     POP_ASSUM MP_TAC THEN
-    ASM_REWRITE_TAC [parse_parse_map; append_stream_def] THEN
-    MP_TAC (ISPECL [`p : (A,B) parser`; `s : A stream`] parse_cases) THEN
+    ASM_REWRITE_TAC [parse_parse_map; append_pstream_def] THEN
+    MP_TAC (ISPECL [`p : (A,B) parser`; `s : A pstream`] parse_cases) THEN
     STRIP_TAC THEN
     ASM_REWRITE_TAC [case_option_def; option_distinct; option_inj; PAIR_EQ] THEN
     STRIP_TAC THEN
@@ -729,15 +729,15 @@ let is_parser_pair = prove
    REPEAT GEN_TAC THEN
    REWRITE_TAC [is_parser_def; parser_pair_def] THEN
    REPEAT GEN_TAC THEN
-   MP_TAC (SPECL [`pb : (A,B) parser`; `x : A`; `xs : A stream`]
+   MP_TAC (SPECL [`pb : (A,B) parser`; `x : A`; `xs : A pstream`]
              dest_parser_cases) THEN
    STRIP_TAC THEN
    ASM_REWRITE_TAC [case_option_def] THEN
-   MP_TAC (ISPECL [`pc : (A,C) parser`; `s' : A stream`]
+   MP_TAC (ISPECL [`pc : (A,C) parser`; `s' : A pstream`]
              parse_cases) THEN
    STRIP_TAC THEN
    ASM_REWRITE_TAC [case_option_def] THEN
-   ASM_MESON_TAC [is_suffix_stream_trans; is_suffix_stream_proper]);;
+   ASM_MESON_TAC [is_suffix_pstream_trans; is_suffix_pstream_proper]);;
 
 export_thm is_parser_pair;;
 
@@ -762,7 +762,7 @@ let parse_parse_pair = prove
              (parse pc s'))
         (parse pb s)`,
     REPEAT STRIP_TAC THEN
-    MP_TAC (ISPEC `s : A stream` stream_cases) THEN
+    MP_TAC (ISPEC `s : A pstream` pstream_cases) THEN
     REPEAT STRIP_TAC THEN
     ASM_REWRITE_TAC [parse_def; case_option_def] THEN
     REWRITE_TAC [dest_parse_pair; parser_pair_def]);;
@@ -780,7 +780,7 @@ let parse_pair_inverse = prove
    REWRITE_TAC [parse_parse_pair] THEN
    MP_TAC (ISPEC `x : B # C` PAIR_SURJECTIVE) THEN
    STRIP_TAC THEN
-   ASM_REWRITE_TAC [append_stream_assoc; case_option_def]);;
+   ASM_REWRITE_TAC [append_pstream_assoc; case_option_def]);;
 
 export_thm parse_pair_inverse;;
 
@@ -797,12 +797,12 @@ let parse_pair_strong_inverse = prove
     POP_ASSUM MP_TAC THEN
     MP_TAC (ISPEC `x : B # C` PAIR_SURJECTIVE) THEN
     STRIP_TAC THEN
-    ASM_REWRITE_TAC [parse_parse_pair; append_stream_assoc] THEN
+    ASM_REWRITE_TAC [parse_parse_pair; append_pstream_assoc] THEN
     MP_TAC (ISPEC `parse (pb : (A,B) parser) s` option_cases) THEN
     STRIP_TAC THEN
     ASM_REWRITE_TAC [case_option_def; option_distinct] THEN
     POP_ASSUM MP_TAC THEN
-    MP_TAC (ISPEC `a : B # A stream` PAIR_SURJECTIVE) THEN
+    MP_TAC (ISPEC `a : B # A pstream` PAIR_SURJECTIVE) THEN
     STRIP_TAC THEN
     ASM_REWRITE_TAC [] THEN
     STRIP_TAC THEN
@@ -810,7 +810,7 @@ let parse_pair_strong_inverse = prove
     STRIP_TAC THEN
     ASM_REWRITE_TAC [case_option_def; option_distinct] THEN
     POP_ASSUM MP_TAC THEN
-    MP_TAC (ISPEC `a' : C # A stream` PAIR_SURJECTIVE) THEN
+    MP_TAC (ISPEC `a' : C # A pstream` PAIR_SURJECTIVE) THEN
     STRIP_TAC THEN
     ASM_REWRITE_TAC [] THEN
     REWRITE_TAC [option_inj; PAIR_EQ] THEN
@@ -839,7 +839,7 @@ export_thm dest_parse_option;;
 let parse_parse_option = prove
   (`!f.
       parse (parse_option (f : A -> B option)) =
-      case_stream
+      case_pstream
         NONE
         NONE
         (\a s. case_option NONE (\b. SOME (b,s)) (f a))`,
@@ -847,9 +847,9 @@ let parse_parse_option = prove
    REWRITE_TAC
      [parse_option_def; parse_parse_partial_map; parse_parse_all] THEN
    REPEAT STRIP_TAC THEN
-   MP_TAC (ISPEC `x : A stream` stream_cases) THEN
+   MP_TAC (ISPEC `x : A pstream` pstream_cases) THEN
    REPEAT STRIP_TAC THEN
-   ASM_REWRITE_TAC [case_stream_def; case_option_def]);;
+   ASM_REWRITE_TAC [case_pstream_def; case_option_def]);;
 
 export_thm parse_parse_option;;
 
@@ -860,7 +860,7 @@ let parse_option_inverse = prove
    REWRITE_TAC [parse_inverse_def] THEN
    REPEAT STRIP_TAC THEN
    ASM_REWRITE_TAC
-     [parse_parse_option; append_stream_def; case_stream_def;
+     [parse_parse_option; append_pstream_def; case_pstream_def;
       case_option_def]);;
 
 export_thm parse_option_inverse;;
@@ -876,10 +876,10 @@ let parse_option_strong_inverse = prove
    [MATCH_MP_TAC parse_option_inverse THEN
     ASM_REWRITE_TAC [];
     POP_ASSUM MP_TAC THEN
-    ASM_REWRITE_TAC [parse_parse_option; append_stream_def] THEN
-    MP_TAC (ISPEC `s : A stream` stream_cases) THEN
+    ASM_REWRITE_TAC [parse_parse_option; append_pstream_def] THEN
+    MP_TAC (ISPEC `s : A pstream` pstream_cases) THEN
     STRIP_TAC THEN
-    ASM_REWRITE_TAC [case_stream_def; option_distinct; stream_inj] THEN
+    ASM_REWRITE_TAC [case_pstream_def; option_distinct; pstream_inj] THEN
     MP_TAC (ISPEC `(f : A -> B option) a0` option_cases) THEN
     STRIP_TAC THEN
     ASM_REWRITE_TAC [case_option_def; option_distinct; option_inj; PAIR_EQ] THEN
@@ -906,171 +906,171 @@ export_thm dest_parse_some;;
 let parse_parse_some = prove
   (`!p.
       parse (parse_some (p : A -> bool)) =
-      case_stream
+      case_pstream
         NONE
         NONE
         (\a s. if p a then SOME (a,s) else NONE)`,
    ONCE_REWRITE_TAC [FUN_EQ_THM] THEN
    REPEAT GEN_TAC THEN
-   MP_TAC (ISPEC `x : A stream` stream_cases) THEN
+   MP_TAC (ISPEC `x : A pstream` pstream_cases) THEN
    STRIP_TAC THEN
-   ASM_REWRITE_TAC [parse_def; case_stream_def; dest_parse_some]);;
+   ASM_REWRITE_TAC [parse_def; case_pstream_def; dest_parse_some]);;
 
 export_thm parse_parse_some;;
 
 logfile "parser-all-def";;
 
-let parse_stream_exists = prove
+let parse_pstream_exists = prove
   (`!(p : (A,B) parser). ?f.
-      (f Error = Error) /\
-      (f Eof = Eof) /\
+      (f ErrorPstream = ErrorPstream) /\
+      (f EofPstream = EofPstream) /\
       (!a s.
-         f (Stream a s) =
+         f (ConsPstream a s) =
            case_option
-             Error
-             (\ (b,s'). Stream b (f s'))
+             ErrorPstream
+             (\ (b,s'). ConsPstream b (f s'))
              (dest_parser p a s))`,
    let exists0 = prove
      (`!(p : (A,B) parser). ?f.
          !s.
            f s =
            (\f'.
-              case_stream
-                Error
-                Eof
+              case_pstream
+                ErrorPstream
+                EofPstream
                 (\a s'.
                    case_option
-                     Error
-                     (\ (b,s''). Stream b (f' s''))
+                     ErrorPstream
+                     (\ (b,s''). ConsPstream b (f' s''))
                      (dest_parser p a s'))) f s`,
       GEN_TAC THEN
-      MATCH_MP_TAC is_proper_suffix_stream_recursion THEN
+      MATCH_MP_TAC is_proper_suffix_pstream_recursion THEN
       SIMP_TAC [] THEN
       REPEAT STRIP_TAC THEN
-      MP_TAC (SPEC `s : A stream` stream_cases) THEN
+      MP_TAC (SPEC `s : A pstream` pstream_cases) THEN
       STRIP_TAC THEN
-      ASM_REWRITE_TAC [case_stream_def] THEN
+      ASM_REWRITE_TAC [case_pstream_def] THEN
       MP_TAC (ISPEC `dest_parser (p : (A,B) parser) a0 a1` option_cases) THEN
       STRIP_TAC THEN
       ASM_REWRITE_TAC [case_option_def] THEN
       POP_ASSUM MP_TAC THEN
-      MP_TAC (ISPEC `a : B # A stream` PAIR_SURJECTIVE) THEN
+      MP_TAC (ISPEC `a : B # A pstream` PAIR_SURJECTIVE) THEN
       STRIP_TAC THEN
-      ASM_REWRITE_TAC [stream_inj] THEN
+      ASM_REWRITE_TAC [pstream_inj] THEN
       STRIP_TAC THEN
       FIRST_ASSUM MATCH_MP_TAC THEN
-      ASM_REWRITE_TAC [is_proper_suffix_stream_def] THEN
-      REWRITE_TAC [GSYM is_suffix_stream_def] THEN
+      ASM_REWRITE_TAC [is_proper_suffix_pstream_def] THEN
+      REWRITE_TAC [GSYM is_suffix_pstream_def] THEN
       MATCH_MP_TAC
-        (ISPECL [`p : (A,B) parser`; `a0 : A`; `a1 : A stream`;
-                 `x : B`; `y : A stream`] dest_parser_suffix_stream) THEN
+        (ISPECL [`p : (A,B) parser`; `a0 : A`; `a1 : A pstream`;
+                 `x : B`; `y : A pstream`] dest_parser_suffix_pstream) THEN
       ASM_REWRITE_TAC []) in
    GEN_TAC THEN
    MP_TAC (SPEC `p : (A,B) parser` exists0) THEN
    STRIP_TAC THEN
-   EXISTS_TAC `f : A stream -> B stream` THEN
+   EXISTS_TAC `f : A pstream -> B pstream` THEN
    REPEAT STRIP_TAC THEN
    POP_ASSUM (fun th -> CONV_TAC (LAND_CONV (REWR_CONV th))) THEN
-   REWRITE_TAC [case_stream_def]);;
+   REWRITE_TAC [case_pstream_def]);;
 
-let (parse_stream_error,
-     parse_stream_eof,
-     parse_stream_stream) =
+let (parse_pstream_error,
+     parse_pstream_eof,
+     parse_pstream_cons) =
   let def =
-    new_specification ["parse_stream"]
-    (REWRITE_RULE [SKOLEM_THM] parse_stream_exists) in
+    new_specification ["parse_pstream"]
+    (REWRITE_RULE [SKOLEM_THM] parse_pstream_exists) in
   CONJ_TRIPLE (REWRITE_RULE [FORALL_AND_THM] def);;
 
-export_thm parse_stream_error;;
-export_thm parse_stream_eof;;
-export_thm parse_stream_stream;;
+export_thm parse_pstream_error;;
+export_thm parse_pstream_eof;;
+export_thm parse_pstream_cons;;
 
-let parse_stream_def =
+let parse_pstream_def =
   REWRITE_RULE [GSYM FORALL_AND_THM]
-    (CONJ parse_stream_error (CONJ parse_stream_eof parse_stream_stream));;
+    (CONJ parse_pstream_error (CONJ parse_pstream_eof parse_pstream_cons));;
 
 logfile "parser-all-thm";;
 
-let parse_stream_append = prove
+let parse_pstream_append = prove
   (`!p (e : A -> B list) x s.
       parse_inverse p e ==>
-      parse_stream p (append_stream (e x) s) = Stream x (parse_stream p s)`,
+      parse_pstream p (append_pstream (e x) s) = ConsPstream x (parse_pstream p s)`,
    REWRITE_TAC [parse_inverse_def] THEN
    REPEAT STRIP_TAC THEN
-   POP_ASSUM (MP_TAC o SPECL [`x : A`; `s : B stream`]) THEN
+   POP_ASSUM (MP_TAC o SPECL [`x : A`; `s : B pstream`]) THEN
    MP_TAC (ISPEC `(e : A -> B list) x` list_CASES) THEN
    STRIP_TAC THENL
-   [ASM_REWRITE_TAC [append_stream_def] THEN
-    MP_TAC (ISPECL [`p : (B,A) parser`; `s : B stream`] parse_cases) THEN
+   [ASM_REWRITE_TAC [append_pstream_def] THEN
+    MP_TAC (ISPECL [`p : (B,A) parser`; `s : B pstream`] parse_cases) THEN
     STRIP_TAC THENL
     [ASM_REWRITE_TAC [option_distinct];
      ASM_REWRITE_TAC [option_inj; PAIR_EQ] THEN
      STRIP_TAC THEN
-     PAT_ASSUM `is_proper_suffix_stream (X : A stream) Y` THEN
-     ASM_REWRITE_TAC [is_proper_suffix_stream_refl]];
-    ASM_REWRITE_TAC [parse_def; parse_stream_def; append_stream_def] THEN
+     PAT_ASSUM `is_proper_suffix_pstream (X : A pstream) Y` THEN
+     ASM_REWRITE_TAC [is_proper_suffix_pstream_refl]];
+    ASM_REWRITE_TAC [parse_def; parse_pstream_def; append_pstream_def] THEN
     STRIP_TAC THEN
     ASM_REWRITE_TAC [case_option_def]]);;
 
-export_thm parse_stream_append;;
+export_thm parse_pstream_append;;
 
-let parse_stream_inverse = prove
+let parse_pstream_inverse = prove
   (`!p (e : A -> B list) l.
       parse_inverse p e ==>
-      parse_stream p (list_to_stream (concat (MAP e l))) =
-      list_to_stream l`,
+      parse_pstream p (list_to_pstream (concat (MAP e l))) =
+      list_to_pstream l`,
    REPEAT STRIP_TAC THEN
    SPEC_TAC (`l : A list`, `l : A list`) THEN
    LIST_INDUCT_TAC THENL
    [REWRITE_TAC
-      [MAP; concat_def; parse_stream_def; list_to_stream_def;
-       append_stream_def];
+      [MAP; concat_def; parse_pstream_def; list_to_pstream_def;
+       append_pstream_def];
     ALL_TAC] THEN
    POP_ASSUM MP_TAC THEN
    REWRITE_TAC
-     [MAP; concat_def; parse_stream_def; list_to_stream_def;
-      append_stream_def] THEN
+     [MAP; concat_def; parse_pstream_def; list_to_pstream_def;
+      append_pstream_def] THEN
    DISCH_THEN (fun th -> REWRITE_TAC [SYM th]) THEN
-   REWRITE_TAC [append_stream_assoc] THEN
-   MATCH_MP_TAC parse_stream_append THEN
+   REWRITE_TAC [append_pstream_assoc] THEN
+   MATCH_MP_TAC parse_pstream_append THEN
    FIRST_ASSUM ACCEPT_TAC);;
 
-export_thm parse_stream_inverse;;
+export_thm parse_pstream_inverse;;
 
-let parse_stream_strong_inverse = prove
+let parse_pstream_strong_inverse = prove
   (`!p (e : A -> B list) s.
       parse_strong_inverse p e ==>
-      case_option T (\l. stream_to_list s = SOME (concat (MAP e l)))
-        (stream_to_list (parse_stream p s))`,
+      case_option T (\l. pstream_to_list s = SOME (concat (MAP e l)))
+        (pstream_to_list (parse_pstream p s))`,
    REPEAT STRIP_TAC THEN
-   SPEC_TAC (`s : B stream`, `s : B stream`) THEN
-   MATCH_MP_TAC is_proper_suffix_stream_induct THEN
+   SPEC_TAC (`s : B pstream`, `s : B pstream`) THEN
+   MATCH_MP_TAC is_proper_suffix_pstream_induct THEN
    GEN_TAC THEN
-   MP_TAC (ISPEC `s : B stream` stream_cases) THEN
+   MP_TAC (ISPEC `s : B pstream` pstream_cases) THEN
    STRIP_TAC THENL
    [POP_ASSUM SUBST_VAR_TAC THEN
-    REWRITE_TAC [stream_to_list_def; parse_stream_def; case_option_def];
+    REWRITE_TAC [pstream_to_list_def; parse_pstream_def; case_option_def];
     POP_ASSUM SUBST_VAR_TAC THEN
     REWRITE_TAC
-      [stream_to_list_def; parse_stream_def; case_option_def; MAP;
+      [pstream_to_list_def; parse_pstream_def; case_option_def; MAP;
        concat_def];
     ALL_TAC] THEN
    POP_ASSUM SUBST_VAR_TAC THEN
    STRIP_TAC THEN
-   REWRITE_TAC [parse_stream_def] THEN
-   MP_TAC (ISPECL [`p : (B,A) parser`; `a0 : B`; `a1 : B stream`]
+   REWRITE_TAC [parse_pstream_def] THEN
+   MP_TAC (ISPECL [`p : (B,A) parser`; `a0 : B`; `a1 : B pstream`]
            dest_parser_cases) THEN
    STRIP_TAC THENL
-   [ASM_REWRITE_TAC [case_option_def; stream_to_list_def];
+   [ASM_REWRITE_TAC [case_option_def; pstream_to_list_def];
     ALL_TAC] THEN
    ASM_REWRITE_TAC [case_option_def] THEN
-   CONV_TAC (RAND_CONV (REWRITE_CONV [stream_to_list_def])) THEN
-   FIRST_X_ASSUM (MP_TAC o SPEC `s' : B stream`) THEN
+   CONV_TAC (RAND_CONV (REWRITE_CONV [pstream_to_list_def])) THEN
+   FIRST_X_ASSUM (MP_TAC o SPEC `s' : B pstream`) THEN
    COND_TAC THENL
-   [PAT_ASSUM `is_suffix_stream (X : B stream) Y` THEN
-    REWRITE_TAC [is_suffix_stream_def; is_proper_suffix_stream_def];
+   [PAT_ASSUM `is_suffix_pstream (X : B pstream) Y` THEN
+    REWRITE_TAC [is_suffix_pstream_def; is_proper_suffix_pstream_def];
     ALL_TAC] THEN
-   MP_TAC (ISPEC `stream_to_list (parse_stream (p : (B,A) parser) s')`
+   MP_TAC (ISPEC `pstream_to_list (parse_pstream (p : (B,A) parser) s')`
            option_cases) THEN
    STRIP_TAC THENL
    [ASM_REWRITE_TAC [case_option_def];
@@ -1078,50 +1078,50 @@ let parse_stream_strong_inverse = prove
    ASM_REWRITE_TAC [case_option_def] THEN
    PAT_ASSUM `parse_strong_inverse (p : (B,A) parser) e` THEN
    REWRITE_TAC [parse_strong_inverse_def] THEN
-   DISCH_THEN (MP_TAC o SPECL [`Stream (a0 : B) a1`; `b : A`;
-                               `s' : B stream`] o CONJUNCT2) THEN
+   DISCH_THEN (MP_TAC o SPECL [`ConsPstream (a0 : B) a1`; `b : A`;
+                               `s' : B pstream`] o CONJUNCT2) THEN
    COND_TAC THENL
    [ASM_REWRITE_TAC [parse_def];
     ALL_TAC] THEN
    DISCH_THEN (fun th -> REWRITE_TAC [th]) THEN
-   REWRITE_TAC [stream_to_list_append] THEN
+   REWRITE_TAC [pstream_to_list_append] THEN
    DISCH_THEN (fun th -> REWRITE_TAC [th]) THEN
    REWRITE_TAC [case_option_def; option_inj; MAP; concat_def]);;
 
-export_thm parse_stream_strong_inverse;;
+export_thm parse_pstream_strong_inverse;;
 
-let parse_stream_length = prove
+let parse_pstream_length = prove
   (`!(p : (A,B) parser) s.
-      length_stream (parse_stream p s) <= length_stream s`,
+      length_pstream (parse_pstream p s) <= length_pstream s`,
    GEN_TAC THEN
-   MATCH_MP_TAC is_proper_suffix_stream_induct THEN
+   MATCH_MP_TAC is_proper_suffix_pstream_induct THEN
    GEN_TAC THEN
-   MP_TAC (ISPEC `s : A stream` stream_cases) THEN
+   MP_TAC (ISPEC `s : A pstream` pstream_cases) THEN
    STRIP_TAC THENL
    [POP_ASSUM SUBST_VAR_TAC THEN
-    REWRITE_TAC [length_stream_def; parse_stream_def; LE_REFL];
+    REWRITE_TAC [length_pstream_def; parse_pstream_def; LE_REFL];
     POP_ASSUM SUBST_VAR_TAC THEN
-    REWRITE_TAC [length_stream_def; parse_stream_def; LE_REFL];
+    REWRITE_TAC [length_pstream_def; parse_pstream_def; LE_REFL];
     ALL_TAC] THEN
    POP_ASSUM SUBST_VAR_TAC THEN
    STRIP_TAC THEN
-   REWRITE_TAC [parse_stream_def] THEN
-   MP_TAC (ISPECL [`p : (A,B) parser`; `a0 : A`; `a1 : A stream`]
+   REWRITE_TAC [parse_pstream_def] THEN
+   MP_TAC (ISPECL [`p : (A,B) parser`; `a0 : A`; `a1 : A pstream`]
            dest_parser_cases) THEN
    STRIP_TAC THENL
-   [ASM_REWRITE_TAC [case_option_def; length_stream_def; LE_0];
+   [ASM_REWRITE_TAC [case_option_def; length_pstream_def; LE_0];
     ALL_TAC] THEN
    ASM_REWRITE_TAC [case_option_def] THEN
-   REWRITE_TAC [length_stream_def; LE_SUC] THEN
+   REWRITE_TAC [length_pstream_def; LE_SUC] THEN
    MATCH_MP_TAC LE_TRANS THEN
-   EXISTS_TAC `length_stream (s' : A stream)` THEN
+   EXISTS_TAC `length_pstream (s' : A pstream)` THEN
    CONJ_TAC THENL
    [FIRST_X_ASSUM MATCH_MP_TAC THEN
-    PAT_ASSUM `is_suffix_stream (X : A stream) Y` THEN
-    REWRITE_TAC [is_suffix_stream_def; is_proper_suffix_stream_def];
-    MATCH_MP_TAC is_suffix_stream_length THEN
+    PAT_ASSUM `is_suffix_pstream (X : A pstream) Y` THEN
+    REWRITE_TAC [is_suffix_pstream_def; is_proper_suffix_pstream_def];
+    MATCH_MP_TAC is_suffix_pstream_length THEN
     FIRST_ASSUM ACCEPT_TAC]);;
 
-export_thm parse_stream_length;;
+export_thm parse_pstream_length;;
 
 logfile_end ();;
