opentheory/haskell/parser.ml
@@ -11,60 +11,61 @@ logfile "haskell-parser-def";;
 
 (* Streams *)
 
-let (streamH_lift_drop,streamH_drop_lift) =
-  let exists = prove (`?(s : A stream). T`, REWRITE_TAC []) in
+let (pstreamH_lift_drop,pstreamH_drop_lift) =
+  let exists = prove (`?(s : A pstream). T`, REWRITE_TAC []) in
   let tybij =
     new_type_definition
-      "streamH" ("lift_streamH","drop_streamH") exists in
+      "pstreamH" ("lift_pstreamH","drop_pstreamH") exists in
   CONJ_PAIR (REWRITE_RULE [] tybij);;
 
-export_thm streamH_lift_drop;;
-export_thm streamH_drop_lift;;
+export_thm pstreamH_lift_drop;;
+export_thm pstreamH_drop_lift;;
 
-let streamH_tybij = CONJ streamH_lift_drop streamH_drop_lift;;
+let pstreamH_tybij = CONJ pstreamH_lift_drop pstreamH_drop_lift;;
 
-let ErrorH_def = new_definition
-  `(ErrorH : A streamH) = lift_streamH Error`;;
+let ErrorPstreamH_def = new_definition
+  `(ErrorPstreamH : A pstreamH) = lift_pstreamH ErrorPstream`;;
 
-export_thm ErrorH_def;;
+export_thm ErrorPstreamH_def;;
 
-let EofH_def = new_definition
-  `(EofH : A streamH) = lift_streamH Eof`;;
+let EofPstreamH_def = new_definition
+  `(EofPstreamH : A pstreamH) = lift_pstreamH EofPstream`;;
 
-export_thm EofH_def;;
+export_thm EofPstreamH_def;;
 
-let StreamH_def = new_definition
-  `!(a : A) s. StreamH a s = lift_streamH (Stream a (drop_streamH s))`;;
+let ConsPstreamH_def = new_definition
+  `!(a : A) s.
+     ConsPstreamH a s = lift_pstreamH (ConsPstream a (drop_pstreamH s))`;;
 
-export_thm StreamH_def;;
+export_thm ConsPstreamH_def;;
 
-let case_streamH_def = new_definition
-  `!(e : B) b f (s : A streamH).
-     case_streamH e b f s =
-     case_stream e b (\a t. f a (lift_streamH t)) (drop_streamH s)`;;
+let case_pstreamH_def = new_definition
+  `!(e : B) b f (s : A pstreamH).
+     case_pstreamH e b f s =
+     case_pstream e b (\a t. f a (lift_pstreamH t)) (drop_pstreamH s)`;;
 
-export_thm case_streamH_def;;
+export_thm case_pstreamH_def;;
 
-let length_streamH_def = new_definition
-  `!(s : A streamH). length_streamH s = length_stream (drop_streamH s)`;;
+let length_pstreamH_def = new_definition
+  `!(s : A pstreamH). length_pstreamH s = length_pstream (drop_pstreamH s)`;;
 
-export_thm length_streamH_def;;
+export_thm length_pstreamH_def;;
 
-let stream_to_listH_def = new_definition
-  `!(s : A streamH). stream_to_listH s = stream_to_list (drop_streamH s)`;;
+let pstream_to_listH_def = new_definition
+  `!(s : A pstreamH). pstream_to_listH s = pstream_to_list (drop_pstreamH s)`;;
 
-export_thm stream_to_listH_def;;
+export_thm pstream_to_listH_def;;
 
-let append_streamH_def = new_definition
-  `!l (s : A streamH).
-     append_streamH l s = lift_streamH (append_stream l (drop_streamH s))`;;
+let append_pstreamH_def = new_definition
+  `!l (s : A pstreamH).
+     append_pstreamH l s = lift_pstreamH (append_pstream l (drop_pstreamH s))`;;
 
-export_thm append_streamH_def;;
+export_thm append_pstreamH_def;;
 
-let list_to_streamH_def = new_definition
-  `!(l : A list). list_to_streamH l = lift_streamH (list_to_stream l)`;;
+let list_to_pstreamH_def = new_definition
+  `!(l : A list). list_to_pstreamH l = lift_pstreamH (list_to_pstream l)`;;
 
-export_thm list_to_streamH_def;;
+export_thm list_to_pstreamH_def;;
 
 (* Parsers *)
 
@@ -82,17 +83,17 @@ let parserH_tybij = CONJ parserH_lift_drop parserH_drop_lift;;
 
 let (lift_parser_resultH_none,lift_parser_resultH_some) =
   let def = new_definition
-    `(lift_parser_resultH : (B # A stream) option ->  (B # A streamH) option) =
+    `(lift_parser_resultH : (B # A pstream) option -> (B # A pstreamH) option) =
        case_option
          NONE
-         (\ (b,s'). SOME (b, lift_streamH s'))` in
+         (\ (b,s'). SOME (b, lift_pstreamH s'))` in
   let th_none = prove
-    (`lift_parser_resultH (NONE : (B # A stream) option) =
-      (NONE : (B # A streamH) option)`,
+    (`lift_parser_resultH (NONE : (B # A pstream) option) =
+      (NONE : (B # A pstreamH) option)`,
      REWRITE_TAC [def; case_option_def])
   and th_some = prove
-    (`!(b : B) (s : A stream).
-         lift_parser_resultH (SOME (b,s)) = SOME (b, lift_streamH s)`,
+    (`!(b : B) (s : A pstream).
+         lift_parser_resultH (SOME (b,s)) = SOME (b, lift_pstreamH s)`,
      REWRITE_TAC [def; case_option_def]) in
   (th_none,th_some);;
 
@@ -104,17 +105,17 @@ let lift_parser_resultH_def =
 
 let (drop_parser_resultH_none,drop_parser_resultH_some) =
   let def = new_definition
-    `(drop_parser_resultH : (B # A streamH) option ->  (B # A stream) option) =
+    `(drop_parser_resultH : (B # A pstreamH) option -> (B # A pstream) option) =
        case_option
          NONE
-         (\ (b,s'). SOME (b, drop_streamH s'))` in
+         (\ (b,s'). SOME (b, drop_pstreamH s'))` in
   let th_none = prove
-    (`drop_parser_resultH (NONE : (B # A streamH) option) =
-      (NONE : (B # A stream) option)`,
+    (`drop_parser_resultH (NONE : (B # A pstreamH) option) =
+      (NONE : (B # A pstream) option)`,
      REWRITE_TAC [def; case_option_def])
   and th_some = prove
-    (`!(b : B) (s : A streamH).
-         drop_parser_resultH (SOME (b,s)) = SOME (b, drop_streamH s)`,
+    (`!(b : B) (s : A pstreamH).
+         drop_parser_resultH (SOME (b,s)) = SOME (b, drop_pstreamH s)`,
      REWRITE_TAC [def; case_option_def]) in
   (th_none,th_some);;
 
@@ -125,21 +126,21 @@ let drop_parser_resultH_def =
     CONJ drop_parser_resultH_none drop_parser_resultH_some;;
 
 let lift_parser_functionH_def = new_definition
-  `!(p : A -> A stream -> (B # A stream) option).
+  `!(p : A -> A pstream -> (B # A pstream) option).
      lift_parser_functionH p =
-     \a s. lift_parser_resultH (p a (drop_streamH s))`;;
+     \a s. lift_parser_resultH (p a (drop_pstreamH s))`;;
 
 export_thm lift_parser_functionH_def;;
 
 let drop_parser_functionH_def = new_definition
-  `!(p : A -> A streamH -> (B # A streamH) option).
+  `!(p : A -> A pstreamH -> (B # A pstreamH) option).
      drop_parser_functionH p =
-     \a s. drop_parser_resultH (p a (lift_streamH s))`;;
+     \a s. drop_parser_resultH (p a (lift_pstreamH s))`;;
 
 export_thm drop_parser_functionH_def;;
 
 let mk_parserH_def = new_definition
-  `!(p : A -> A streamH -> (B # A streamH) option).
+  `!(p : A -> A pstreamH -> (B # A pstreamH) option).
      mk_parserH p = lift_parserH (mk_parser (drop_parser_functionH p))`;;
 
 export_thm mk_parserH_def;;
@@ -153,12 +154,12 @@ export_thm dest_parserH_def;;
 let parseH_def = new_definition
   `!(p : (A,B) parserH) s.
      parseH p s =
-     lift_parser_resultH (parse (drop_parserH p) (drop_streamH s))`;;
+     lift_parser_resultH (parse (drop_parserH p) (drop_pstreamH s))`;;
 
 export_thm parseH_def;;
 
 let parser_noneH_def = new_definition
-  `(parser_noneH : A -> A streamH -> (B # A streamH) option) =
+  `(parser_noneH : A -> A pstreamH -> (B # A pstreamH) option) =
    lift_parser_functionH parser_none`;;
 
 export_thm parser_noneH_def;;
@@ -169,7 +170,7 @@ let parse_noneH_def = new_definition
 export_thm parse_noneH_def;;
 
 let parser_allH_def = new_definition
-  `(parser_allH : A -> A streamH -> (A # A streamH) option) =
+  `(parser_allH : A -> A pstreamH -> (A # A pstreamH) option) =
    lift_parser_functionH parser_all`;;
 
 export_thm parser_allH_def;;
@@ -225,12 +226,12 @@ let parse_someH_def = new_definition
 
 export_thm parse_someH_def;;
 
-let parse_streamH_def = new_definition
+let parse_pstreamH_def = new_definition
   `!(p : (A,B) parserH) s.
-     parse_streamH p s =
-     lift_streamH (parse_stream (drop_parserH p) (drop_streamH s))`;;
+     parse_pstreamH p s =
+     lift_pstreamH (parse_pstream (drop_parserH p) (drop_pstreamH s))`;;
 
-export_thm parse_streamH_def;;
+export_thm parse_pstreamH_def;;
 
 (* ------------------------------------------------------------------------- *)
 (* Properties of Haskell parsers and streams.                                *)
@@ -241,66 +242,66 @@ logfile "haskell-parser-thm";;
 (* Parsers *)
 
 let parser_resultH_drop_lift = prove
- (`!(r : (B # A stream) option).
+ (`!(r : (B # A pstream) option).
      drop_parser_resultH (lift_parser_resultH r) = r`,
   GEN_TAC THEN
-  MP_TAC (ISPEC `r : (B # A stream) option` option_cases) THEN
+  MP_TAC (ISPEC `r : (B # A pstream) option` option_cases) THEN
   STRIP_TAC THENL
   [FIRST_X_ASSUM SUBST_VAR_TAC THEN
    REWRITE_TAC [lift_parser_resultH_def; drop_parser_resultH_def];
    ALL_TAC] THEN
   FIRST_X_ASSUM SUBST_VAR_TAC THEN
-  MP_TAC (ISPEC `a : B # A stream` PAIR_SURJECTIVE) THEN
+  MP_TAC (ISPEC `a : B # A pstream` PAIR_SURJECTIVE) THEN
   STRIP_TAC THEN
   FIRST_X_ASSUM SUBST_VAR_TAC THEN
   REWRITE_TAC
-    [lift_parser_resultH_def; drop_parser_resultH_def; streamH_drop_lift]);;
+    [lift_parser_resultH_def; drop_parser_resultH_def; pstreamH_drop_lift]);;
 
 export_thm parser_resultH_drop_lift;;
 
 let parser_resultH_lift_drop = prove
- (`!(r : (B # A streamH) option).
+ (`!(r : (B # A pstreamH) option).
      lift_parser_resultH (drop_parser_resultH r) = r`,
   GEN_TAC THEN
-  MP_TAC (ISPEC `r : (B # A streamH) option` option_cases) THEN
+  MP_TAC (ISPEC `r : (B # A pstreamH) option` option_cases) THEN
   STRIP_TAC THENL
   [FIRST_X_ASSUM SUBST_VAR_TAC THEN
    REWRITE_TAC [lift_parser_resultH_def; drop_parser_resultH_def];
    ALL_TAC] THEN
   FIRST_X_ASSUM SUBST_VAR_TAC THEN
-  MP_TAC (ISPEC `a : B # A streamH` PAIR_SURJECTIVE) THEN
+  MP_TAC (ISPEC `a : B # A pstreamH` PAIR_SURJECTIVE) THEN
   STRIP_TAC THEN
   FIRST_X_ASSUM SUBST_VAR_TAC THEN
   REWRITE_TAC
-    [lift_parser_resultH_def; drop_parser_resultH_def; streamH_lift_drop]);;
+    [lift_parser_resultH_def; drop_parser_resultH_def; pstreamH_lift_drop]);;
 
 export_thm parser_resultH_lift_drop;;
 
 let parser_functionH_drop_lift = prove
- (`!(p : A -> A stream -> (B # A stream) option).
+ (`!(p : A -> A pstream -> (B # A pstream) option).
      drop_parser_functionH (lift_parser_functionH p) = p`,
   GEN_TAC THEN
   CONV_TAC (REWR_CONV FUN_EQ_THM) THEN
   X_GEN_TAC `a : A` THEN
   CONV_TAC (REWR_CONV FUN_EQ_THM) THEN
-  X_GEN_TAC `s : A stream` THEN
+  X_GEN_TAC `s : A pstream` THEN
   REWRITE_TAC
     [lift_parser_functionH_def; drop_parser_functionH_def;
-     streamH_drop_lift; parser_resultH_drop_lift]);;
+     pstreamH_drop_lift; parser_resultH_drop_lift]);;
 
 export_thm parser_functionH_drop_lift;;
 
 let parser_functionH_lift_drop = prove
- (`!(p : A -> A streamH -> (B # A streamH) option).
+ (`!(p : A -> A pstreamH -> (B # A pstreamH) option).
      lift_parser_functionH (drop_parser_functionH p) = p`,
   GEN_TAC THEN
   CONV_TAC (REWR_CONV FUN_EQ_THM) THEN
   X_GEN_TAC `a : A` THEN
   CONV_TAC (REWR_CONV FUN_EQ_THM) THEN
-  X_GEN_TAC `s : A streamH` THEN
+  X_GEN_TAC `s : A pstreamH` THEN
   REWRITE_TAC
     [lift_parser_functionH_def; drop_parser_functionH_def;
-     streamH_lift_drop; parser_resultH_lift_drop]);;
+     pstreamH_lift_drop; parser_resultH_lift_drop]);;
 
 export_thm parser_functionH_lift_drop;;
 
@@ -331,60 +332,61 @@ logfile "haskell-parser-src";;
 (* Streams *)
 
 let () = (export_haskell_thm o prove)
- (`(!e b (f : A -> A streamH -> B). case_streamH e b f ErrorH = e) /\
-   (!e b (f : A -> A streamH -> B). case_streamH e b f EofH = b) /\
-   (!e b (f : A -> A streamH -> B) a s.
-      case_streamH e b f (StreamH a s) = f a s)`,
+ (`(!e b (f : A -> A pstreamH -> B). case_pstreamH e b f ErrorPstreamH = e) /\
+   (!e b (f : A -> A pstreamH -> B). case_pstreamH e b f EofPstreamH = b) /\
+   (!e b (f : A -> A pstreamH -> B) a s.
+      case_pstreamH e b f (ConsPstreamH a s) = f a s)`,
   REWRITE_TAC
-    [case_streamH_def; ErrorH_def; EofH_def; StreamH_def; case_stream_def;
-     streamH_tybij]);;
+    [case_pstreamH_def; ErrorPstreamH_def; EofPstreamH_def; ConsPstreamH_def;
+     case_pstream_def; pstreamH_tybij]);;
 
 let () = (export_haskell_thm o prove)
- (`length_streamH (ErrorH : A streamH) = 0 /\
-   length_streamH (EofH : A streamH) = 0 /\
-   (!(a:A) s. length_streamH (StreamH a s) = length_streamH s + 1)`,
+ (`length_pstreamH (ErrorPstreamH : A pstreamH) = 0 /\
+   length_pstreamH (EofPstreamH : A pstreamH) = 0 /\
+   (!(a:A) s. length_pstreamH (ConsPstreamH a s) = length_pstreamH s + 1)`,
   REWRITE_TAC
-    [length_streamH_def; ErrorH_def; EofH_def; StreamH_def; streamH_tybij;
-     length_stream_def; ADD1]);;
+    [length_pstreamH_def; ErrorPstreamH_def; EofPstreamH_def; ConsPstreamH_def;
+     pstreamH_tybij; length_pstream_def; ADD1]);;
 
 let () = (export_haskell_thm o prove)
- (`stream_to_listH (ErrorH : A streamH) = NONE /\
-   stream_to_listH (EofH : A streamH) = SOME [] /\
+ (`pstream_to_listH (ErrorPstreamH : A pstreamH) = NONE /\
+   pstream_to_listH (EofPstreamH : A pstreamH) = SOME [] /\
    (!(a : A) s.
-      stream_to_listH (StreamH a s) =
-      case_option NONE (\l. SOME (CONS a l)) (stream_to_listH s))`,
+      pstream_to_listH (ConsPstreamH a s) =
+      case_option NONE (\l. SOME (CONS a l)) (pstream_to_listH s))`,
   REWRITE_TAC
-    [stream_to_listH_def; ErrorH_def; EofH_def; StreamH_def; streamH_tybij;
-     stream_to_list_def]);;
+    [pstream_to_listH_def; ErrorPstreamH_def; EofPstreamH_def; ConsPstreamH_def;
+     pstreamH_tybij; pstream_to_list_def]);;
 
 let () = (export_haskell_thm o prove)
- (`(!(s : A streamH). append_streamH [] s = s) /\
+ (`(!(s : A pstreamH). append_pstreamH [] s = s) /\
    (!(h : A) t s.
-      append_streamH (CONS h t) s = StreamH h (append_streamH t s))`,
+      append_pstreamH (CONS h t) s = ConsPstreamH h (append_pstreamH t s))`,
   REWRITE_TAC
-    [append_streamH_def; streamH_tybij; StreamH_def; append_stream_def]);;
+    [append_pstreamH_def; pstreamH_tybij; ConsPstreamH_def;
+     append_pstream_def]);;
 
 let () = (export_haskell_thm o prove)
- (`!(l : A list). list_to_streamH l = append_streamH l EofH`,
+ (`!(l : A list). list_to_pstreamH l = append_pstreamH l EofPstreamH`,
   REWRITE_TAC
-    [list_to_streamH_def; streamH_tybij; EofH_def; list_to_stream_def;
-     append_streamH_def]);;
+    [list_to_pstreamH_def; pstreamH_tybij; EofPstreamH_def; list_to_pstream_def;
+     append_pstreamH_def]);;
 
 (* Parsers *)
 
 let () = export_haskell_thm parserH_mk_dest;;
 
 let () = (export_haskell_thm o prove)
- (`(!(p : (A,B) parserH). parseH p ErrorH = NONE) /\
-   (!(p : (A,B) parserH). parseH p EofH = NONE) /\
-   (!(p : (A,B) parserH) a s. parseH p (StreamH a s) = dest_parserH p a s)`,
+ (`(!(p : (A,B) parserH). parseH p ErrorPstreamH = NONE) /\
+   (!(p : (A,B) parserH). parseH p EofPstreamH = NONE) /\
+   (!(p : (A,B) parserH) a s. parseH p (ConsPstreamH a s) = dest_parserH p a s)`,
   REWRITE_TAC
-    [parseH_def; ErrorH_def; EofH_def; StreamH_def; streamH_drop_lift;
-     parse_def; lift_parser_resultH_def; dest_parserH_def;
+    [parseH_def; ErrorPstreamH_def; EofPstreamH_def; ConsPstreamH_def;
+     pstreamH_drop_lift; parse_def; lift_parser_resultH_def; dest_parserH_def;
      lift_parser_functionH_def]);;
 
 let () = (export_haskell_thm o prove)
- (`!a s. parser_noneH a s = (NONE : (B # A streamH) option)`,
+ (`!a s. parser_noneH a s = (NONE : (B # A pstreamH) option)`,
   REWRITE_TAC
     [parser_noneH_def; lift_parser_functionH_def; parser_none_def;
      lift_parser_resultH_def]);;
@@ -399,7 +401,7 @@ let () = (export_haskell_thm o prove)
  (`!(a : A) s. parser_allH a s = SOME (a,s)`,
   REWRITE_TAC
     [parser_allH_def; lift_parser_functionH_def; parser_all_def;
-     lift_parser_resultH_def; streamH_lift_drop]);;
+     lift_parser_resultH_def; pstreamH_lift_drop]);;
 
 let () = (export_haskell_thm o prove)
  (`(parse_allH : (A,A) parserH) = mk_parserH parser_allH`,
@@ -419,7 +421,7 @@ let () = (export_haskell_thm o prove)
     [parser_partial_mapH_def; lift_parser_functionH_def; dest_parserH_def;
      parser_partial_map_def] THEN
   MP_TAC (ISPECL [`drop_parserH (p : (A,B) parserH)`; `a : A`;
-                  `drop_streamH s : A stream`] dest_parser_cases) THEN
+                  `drop_pstreamH s : A pstream`] dest_parser_cases) THEN
   STRIP_TAC THEN
   FIRST_X_ASSUM SUBST1_TAC THEN
   REWRITE_TAC [lift_parser_resultH_def; case_option_def] THEN
@@ -457,13 +459,13 @@ let () = (export_haskell_thm o prove)
     [parser_pairH_def; lift_parser_functionH_def; dest_parserH_def;
      parser_pair_def] THEN
   MP_TAC (ISPECL [`drop_parserH (pb : (A,B) parserH)`; `a : A`;
-                  `drop_streamH s : A stream`] dest_parser_cases) THEN
+                  `drop_pstreamH s : A pstream`] dest_parser_cases) THEN
   STRIP_TAC THEN
   FIRST_X_ASSUM SUBST1_TAC THEN
   REWRITE_TAC [lift_parser_resultH_def; case_option_def] THEN
-  REWRITE_TAC [parseH_def; streamH_drop_lift] THEN
+  REWRITE_TAC [parseH_def; pstreamH_drop_lift] THEN
   MP_TAC (ISPECL [`drop_parserH (pc : (A,C) parserH)`;
-                  `s' : A stream`] parse_cases) THEN
+                  `s' : A pstream`] parse_cases) THEN
   STRIP_TAC THEN
   FIRST_X_ASSUM SUBST1_TAC THEN
   REWRITE_TAC [lift_parser_resultH_def; case_option_def]);;
@@ -495,23 +497,24 @@ let () = (export_haskell_thm o prove)
     [parse_someH_def; parse_optionH_def; parse_some_def]);;
 
 let () = (export_haskell_thm o prove)
- (`(!(p : (A,B) parserH). parse_streamH p ErrorH = ErrorH) /\
-   (!(p : (A,B) parserH). parse_streamH p EofH = EofH) /\
+ (`(!(p : (A,B) parserH). parse_pstreamH p ErrorPstreamH = ErrorPstreamH) /\
+   (!(p : (A,B) parserH). parse_pstreamH p EofPstreamH = EofPstreamH) /\
    (!(p : (A,B) parserH) a s.
-      parse_streamH p (StreamH a s) =
+      parse_pstreamH p (ConsPstreamH a s) =
       case_option
-        ErrorH
-        (\ (b,s'). StreamH b (parse_streamH p s'))
+        ErrorPstreamH
+        (\ (b,s'). ConsPstreamH b (parse_pstreamH p s'))
         (dest_parserH p a s))`,
   REWRITE_TAC
-    [parse_streamH_def; ErrorH_def; EofH_def; StreamH_def; streamH_drop_lift;
-     parse_stream_def; dest_parserH_def; lift_parser_functionH_def] THEN
+    [parse_pstreamH_def; ErrorPstreamH_def; EofPstreamH_def; ConsPstreamH_def;
+     pstreamH_drop_lift; parse_pstream_def; dest_parserH_def;
+     lift_parser_functionH_def] THEN
   REPEAT GEN_TAC THEN
   MP_TAC (ISPECL [`drop_parserH (p : (A,B) parserH)`; `a : A`;
-                  `drop_streamH s : A stream`] dest_parser_cases) THEN
+                  `drop_pstreamH s : A pstream`] dest_parser_cases) THEN
   STRIP_TAC THEN
   FIRST_X_ASSUM SUBST1_TAC THEN
-  REWRITE_TAC [lift_parser_resultH_def; case_option_def; streamH_drop_lift]);;
+  REWRITE_TAC [lift_parser_resultH_def; case_option_def; pstreamH_drop_lift]);;
 
 (* ------------------------------------------------------------------------- *)
 (* Testing.                                                                  *)
@@ -524,29 +527,29 @@ logfile "haskell-parser-test";;
 let () = (export_haskell_thm o prove)
  (`!(l : A list) s.
      equal_numH
-       (length_streamH (append_streamH l s))
-       (LENGTH l + length_streamH s)`,
+       (length_pstreamH (append_pstreamH l s))
+       (LENGTH l + length_pstreamH s)`,
   REWRITE_TAC
-    [length_streamH_def; append_streamH_def; streamH_drop_lift;
-     append_stream_length; equal_numH_def]);;
+    [length_pstreamH_def; append_pstreamH_def; pstreamH_drop_lift;
+     append_pstream_length; equal_numH_def]);;
 
 let () = (export_haskell_thm o prove)
  (`!(l : num list).
      equal_optionH (equal_listH equal_numH)
-       (stream_to_listH (list_to_streamH l)) (SOME l)`,
+       (pstream_to_listH (list_to_pstreamH l)) (SOME l)`,
   REWRITE_TAC
     [equal_numH_def; equal_listH; equal_optionH;
-     stream_to_listH_def; list_to_streamH_def; streamH_drop_lift;
-     list_to_stream_to_list]);;
+     pstream_to_listH_def; list_to_pstreamH_def; pstreamH_drop_lift;
+     list_to_pstream_to_list]);;
 
 (***
-export_haskell_thm append_stream_assoc;;
+export_haskell_thm append_pstream_assoc;;
 
-export_haskell_thm stream_to_list_append;;
+export_haskell_thm pstream_to_list_append;;
 
-export_haskell_thm list_to_stream_length;;
+export_haskell_thm list_to_pstream_length;;
 
-export_haskell_thm stream_to_list_length;;
+export_haskell_thm pstream_to_list_length;;
 
 (* Parsers *)
 ***)
